{
 "cells": [
  {
   "cell_type": "code",
   "execution_count": null,
   "id": "6187ab4c",
   "metadata": {},
   "outputs": [],
   "source": [
    "# ||A||_F = ||u||_2||v||_2\n",
    "# Proof:\n",
    "# The Frobenius norm of matrix A is given by\n",
    "# ||A||_F = sqrt(Σ_(i,j)A_(i,j)^2)\n",
    "#         = sqrt(Σ_(i,j)(uv^T)_(i,j)^2)\n",
    "#         = sqrt(Σ_(i,j)(u_iv_j)^2)\n",
    "#         = sqrt(Σ_(i,j)u_i^2v_j^2 )\n",
    "#         = sqrt(Σ_i u_i^2 Σ_j v_j^2)\n",
    "#         = sqrt(||u||_2^2||v||_2^2)\n",
    "#         = ||u||_2||v||_2\n",
    "\n",
    "# Therefore, ||A||_F = ||u||_2||v||_2\n",
    "\n",
    "\n",
    "# ||A||_2 = ||u||_2||v||_2\n",
    "\n",
    "\n",
    "# Proof:\n",
    "\n",
    "# Let A = uv^T.\n",
    "\n",
    "# Then, ||A||_2 = ||uv^T||_2\n",
    "\n",
    "# By the definition of matrix norm,\n",
    "\n",
    "# ||uv^T||_2 = max |u^Tv|\n",
    "\n",
    "# Since |u^Tv| = ||u||_2||v||_2,\n",
    "\n",
    "# max |u^Tv| = ||u||_2||v||_2\n",
    "\n",
    "# Therefore,\n",
    "\n",
    "# ||A||_2 = ||uv^T||_2 = ||u||_2||v||_2\n",
    "\n",
    "\n",
    "\n",
    "# ||A||_∞ = ||u||_∞||v||_1\n",
    "\n",
    "\n",
    "# Proof:\n",
    "\n",
    "# We can write A as:\n",
    "# A = uv^T = [u_1, u_2, ..., u_m] [v_1, v_2, ..., v_m]^T\n",
    "\n",
    "# By definition, the max-norm of A is the maximum absolute row sum of A, i.e.\n",
    "# ||A||_∞ = max {|u_1v_1 + u_2v_2 + ... + u_mv_m|, |u_1v_2 + u_2v_2 + ... + u_mv_m|, ... , |u_1v_m + u_2v_m + ... + u_mv_m|}\n",
    "\n",
    "# The maximum absolute row sum can be rewritten as:\n",
    "# ||A||_∞ = max {|u_1||v_1| + |u_2||v_2| + ... + |u_m||v_m|}\n",
    "\n",
    "# By definition, the 1-norm of a vector is the maximum absolute column sum of the vector, i.e.\n",
    "# ||v||_1 = max{|v_1| + |v_2| + ... + |v_m|}\n",
    "\n",
    "# Substituting this into the expression for the max-norm of A yields:\n",
    "# ||A||_∞ = max {|u_1||v_1| + |u_2||v_2| + ... + |u_m||v_m|} = max {|u_1|}*(|v_1| + |v_2| + ... + |v_m|) = ||u||_∞||v||_1\n",
    "\n",
    "# Therefore, ||A||_∞ = ||u||_∞||v||_1\n",
    "\n",
    "\n",
    "\n",
    "\n",
    "\n",
    "\n",
    "\n",
    "\n",
    "# ||A||_1 = ||u||_1||v||_∞\n",
    "\n",
    "\n",
    "# Proof:\n",
    "# We know that ||A||_1 = max_i (sum_j |A_ij|). By definition of matrix A, A_ij = u_i v_j. \n",
    "# Therefore, \n",
    "# ||A||_1 = max_i (sum_j |u_i v_j|)\n",
    "#           = max_i (sum_j |u_i||v_j|)\n",
    "#           = max_i (|u_i| sum_j |v_j|)\n",
    "#           = max_i (|u_i||v_j|), for j = argmax_j |v_j|\n",
    "#           = ||u||_1 ||v||_∞\n",
    "\n",
    "\n",
    "\n",
    "# Suppose A = uv^T for some vectors u; v 2 R^m. Show the following identities for the norms of A\n",
    "# ||A||_1 = ||u||_1||v||_∞\n",
    "\n",
    "\n",
    "# ||A||_1 = max_iΣ|A_ij| \n",
    "#         = max_i (Σ|u_i v_j| ) \n",
    "#         = max_i (|u_i| Σ|v_j| ) \n",
    "#         = ||u||_1 ||v||_∞\n",
    "        \n"
   ]
  },
  {
   "cell_type": "code",
   "execution_count": null,
   "id": "f19a942c",
   "metadata": {},
   "outputs": [],
   "source": [
    "# (a) Show that if a matrix Q is orthogonal and lower triangular, then it is diagonal.\n",
    "# Hint: One way to proceed is to note that QQ^T = I, where I is the identity matrix. Perform\n",
    "# forward substitution on this system, treating Q^T as an unknown, and show you can't get an\n",
    "# upper triangular matrix.\n",
    "\n",
    "\n",
    "# Let Q be an orthogonal and lower triangular matrix. We have QQ^T = I. Rearranging, we get Q^T = Q^TQ.\n",
    "\n",
    "# Since Q is lower triangular, it can be written as:\n",
    "# Q =  # this is not a lower triangular matrix, check!\n",
    "# [a b c\n",
    "#  0 d e\n",
    "#  0 0 f]\n",
    "\n",
    "# We can then perform forward substitution on the system, treating Q^T as an unknown.\n",
    "\n",
    "# Q^T =\n",
    "# [a 0 0\n",
    "#  b d 0 \n",
    "#  c e f]\n",
    "\n",
    "# Substituting this back into Q^TQ, we get:\n",
    "\n",
    "# [a 0 0\n",
    "#  b d 0 \n",
    "#  c e f] * \n",
    "# [a b c\n",
    "#  0 d e\n",
    "#  0 0 f] \n",
    "\n",
    "# =\n",
    "# [a^2 b*c 0\n",
    "# b*d d^2 e*f\n",
    "# c*e e*f f^2]\n",
    "\n",
    "# We can see that this is not an upper triangular matrix, so the only solution is for the diagonal elements of Q to be the same as the diagonal elements of Q^T. Thus, Q is diagonal."
   ]
  },
  {
   "cell_type": "code",
   "execution_count": null,
   "id": "40a5237a",
   "metadata": {},
   "outputs": [],
   "source": [
    "# Suppose Q is an orthogonal lower triangular matrix and let Q^T be the transpose of Q.  Then QQ^T = I, where I is the identity matrix.\n",
    "\n",
    "# We can perform forward substitution to solve for Q^T.  First, we have \n",
    "# Q_{11}Q^T_{11} = I_{11}\n",
    "# so Q^T_{11} = 1/Q_{11}.\n",
    "\n",
    "# Now, for the rest of the entries, we have\n",
    "# Q_{12}Q^T_{11} + Q_{22}Q^T_{22} = I_{22}\n",
    "# Substituting in the value of Q^T_{11} derived above, this reduces to\n",
    "# Q_{12}/Q_{11} + Q_{22}Q^T_{22} = I_{22}.\n",
    "# Re-arranging, this gives\n",
    "# Q_{22}Q^T_{22} = I_{22} - Q_{12}/Q_{11}\n",
    "# and thus Q^T_{22} = 1/Q_{22} (I_{22} - Q_{12}/Q_{11}).\n",
    "\n",
    "# Continuing in this way, we can solve for each entry of Q^T in terms of entries of Q.  However, it is easy to see that each entry of Q^T is a function of entries of Q in either the same row or the same column.  Therefore, Q^T is a lower triangular matrix, and thus Q is a diagonal matrix.\n"
   ]
  },
  {
   "cell_type": "code",
   "execution_count": null,
   "id": "e43f9f52",
   "metadata": {},
   "outputs": [],
   "source": [
    "# Proof:\n",
    "# Let Q be an orthogonal and lower triangular matrix. We know that QQ^T = I, where I is the identity matrix. To prove that Q is diagonal, we will show that Q^T is also lower triangular.\n",
    "\n",
    "# We can rewrite the equation QQ^T = I as \n",
    "\n",
    "# (Q_11)(Q^T_11) + (Q_12)(Q^T_21) + ... + (Q_1n)(Q^T_n1) = 1\n",
    "\n",
    "# (Q_21)(Q^T_11) + (Q_22)(Q^T_21) + ... + (Q_2n)(Q^T_n1) = 0\n",
    "\n",
    "# ...\n",
    "\n",
    "# (Q_n1)(Q^T_11) + (Q_n2)(Q^T_21) + ... + (Q_nn)(Q^T_n1) = 0\n",
    "\n",
    "# We can solve this system of equations by performing forward substitution. We start with the first equation and solve for Q_11^T.\n",
    "\n",
    "# Q_11^T = (1 - (Q_12)(Q^T_21) - ... - (Q_1n)(Q^T_n1)) / (Q_11).\n",
    "\n",
    "# Then, we substitute this value into the second equation and solve for Q_12^T.\n",
    "\n",
    "# Q_12^T = (0 - (Q_22)(Q^T_21) - ... - (Q_2n)(Q^T_n1)) / (Q_12).\n",
    "\n",
    "# We continue this process until we solve for all of the elements in Q^T. Since the first element in each equation is the only element that is not multiplied by a zero, we can see that each element in Q^T will be lower triangular. Therefore, Q is diagonal.\n",
    "\n"
   ]
  }
 ],
 "metadata": {
  "kernelspec": {
   "display_name": "ipykernel",
   "language": "python",
   "name": "python3"
  },
  "language_info": {
   "codemirror_mode": {
    "name": "ipython",
    "version": 3
   },
   "file_extension": ".py",
   "mimetype": "text/x-python",
   "name": "python",
   "nbconvert_exporter": "python",
   "pygments_lexer": "ipython3",
   "version": "3.9.12"
  }
 },
 "nbformat": 4,
 "nbformat_minor": 5
}
